Work on mailbox patterns and mailbox configs

theories/TypeSyntax.v
@@ -1,15 +1,105 @@
 (** * Type syntax of mailbox types *)
 
-(** Mailbox type definition *)
-Inductive MType : Type :=
-    MTOutput : MType
-  | MTInput  : MType.
+From MailboxTypes Require Import Message.
+Open Scope mailbox_config_scope.
 
-(** Mailbox pattern definition *)
-Inductive MPattern : Type :=
+Generalizable All Variables.
+
+Section MPattern_defs.
+
+Context `{MessageInterface : IMessage Message}.
+
+(**
+  Mailbox pattern definition.
+  A mailbox pattern is accompanied by the message type
+  [Message], i.e. what kind of messages are inside the mailbox.
+*)
+Inductive MPattern `{IMessage Message} : Type :=
     MPZero : MPattern
   | MPOne : MPattern
-  | MPMessage : MPattern
+  | MPMessage : Message -> MPattern
   | MPChoice : MPattern -> MPattern -> MPattern
   | MPComp : MPattern -> MPattern -> MPattern
   | MPStar : MPattern -> MPattern.
+
+(** Repeated choice a mailbox pattern *)
+Fixpoint Pow (p : MPattern) (n : nat) : MPattern :=
+  match n with
+  | 0 => MPOne
+  | S n => MPChoice p (Pow p n)
+  end.
+
+(**
+   The semantics of mailbox patterns are defined by a relation
+   between a mailbox config and a pattern.
+*)
+Inductive valueOf : MailboxConfig -> MPattern -> Prop :=
+    MPValueOne : valueOf EmptyMailbox MPOne
+  | MPValueMessage : forall m, valueOf (SingletonMailbox m) (MPMessage m)
+  | MPValueChoiceLeft : forall p1 p2 m, valueOf m p1 -> valueOf m (MPChoice p1 p2)
+  | MPValueChoiceRight : forall p1 p2 m, valueOf m p2 -> valueOf m (MPChoice p1 p2)
+  | MPValueComp : forall p1 p2 m a b, valueOf a p1 -> valueOf b p2 -> m =ᵐᵇ (a ⊎ b) -> valueOf m (MPComp p1 p2)
+  | MPValueStar : forall p m, (exists n, valueOf m (Pow p n)) -> valueOf m (MPStar p).
+
+Definition MPInclusion (e f : MPattern) : Prop :=
+  forall m, valueOf m e -> valueOf m f.
+
+Definition MPEqual (e f : MPattern) : Prop :=
+  MPInclusion e f /\ MPInclusion f e.
+
+Lemma MPZero_empty : forall m, ~ (valueOf m MPZero).
+Proof.
+  intros m.
+  destruct m.
+  unfold not; intros valueOf; inversion valueOf.
+Qed.
+End MPattern_defs.
+
+(** Notation on mailbox pattern. Basically the same as in the paper. *)
+Declare Scope mailbox_pattern_scope.
+Open Scope mailbox_pattern_scope.
+
+Notation "𝟘" := MPZero : mailbox_pattern_scope.
+Notation "𝟙" := MPOne : mailbox_pattern_scope.
+Infix "⊕" := MPChoice (at level 66, left associativity) : mailbox_pattern_scope.
+Infix "⊙" := MPComp (at level 65, left associativity) : mailbox_pattern_scope.
+Notation "⋆ E" := (MPStar E) (at level 64) : mailbox_pattern_scope.
+Notation "« M »" := (MPMessage M) : mailbox_pattern_scope.
+Infix "∈" := valueOf (at level 67, left associativity) : mailbox_pattern_scope.
+
+Require Import String.
+Open Scope string_scope.
+
+Lemma Test : ⟨⟩ ∈ (𝟙 ⊕ 𝟘).
+Proof.
+  apply MPValueChoiceLeft.
+  apply MPValueOne.
+Qed.
+
+Lemma Test1 : (⟨ "m" ⟩ ⊎ ⟨ "n" ⟩) ∈ (« "n" » ⊙ « "m" »).
+Proof.
+  eapply MPValueComp.
+  - apply MPValueMessage.
+  - apply MPValueMessage.
+  - now rewrite mailbox_union_comm.
+Qed.
+
+(* TODO
+Lemma Test2 : MPEqual (𝟙 ⊕ 𝟘 ⊕ (« "m" » ⊙ « "n" »)) (𝟙 ⊕ (« "n" » ⊙ « "m" »)).
+Proof.
+  unfold MPEqual.
+  split.
+  - unfold MPInclusion.
+    intros m E.
+*)
+
+Section mailbox_type_def.
+
+Context `{M : IMessage Message}.
+
+(** Mailbox type definition *)
+Inductive MType `{IMessage Message} : Type :=
+    MTOutput : MPattern -> MType
+  | MTInput  : MPattern -> MType.
+
+End mailbox_type_def.
