theories/Message.v
@@ -1,0 +1,102 @@
+(** * Definition of messages *)
+
+Require Import Setoid.
+Require Import Sets.Multiset.
+
+Section Message_def.
+
+(** A message is a type with decidable equality *)
+Class IMessage Message : Type :=
+  {
+    message_eq: Message -> Message -> Prop;
+    message_eq_equiv : Equivalence message_eq;
+    message_eq_dec : forall m n, {message_eq m n} + {~ message_eq m n};
+  }.
+
+End Message_def.
+
+Section MessageConfig_def.
+
+Generalizable All Variables.
+
+Context `{IM : IMessage Message}.
+
+(** A mailbox configuration is a multiset of messages *)
+Definition MailboxConfig := multiset Message.
+
+Definition EmptyMailbox := EmptyBag Message.
+Definition SingletonMailbox (m : Message) := SingletonBag message_eq message_eq_dec m.
+
+Definition mailbox_union (m1 m2 : MailboxConfig) := munion m1 m2.
+Definition mailbox_eq (m1 m2 : MailboxConfig) := meq m1 m2.
+
+Global Instance mailbox_eq_Equiv : Equivalence mailbox_eq.
+Proof.
+  constructor.
+  - unfold Reflexive; apply meq_refl.
+  - unfold Symmetric; apply meq_sym.
+  - unfold Transitive; apply meq_trans.
+Defined.
+
+Lemma mailbox_union_comm : forall m1 m2, mailbox_eq (mailbox_union m1 m2) (mailbox_union m2 m1).
+Proof.
+  unfold mailbox_union; unfold mailbox_eq; apply munion_comm.
+Qed.
+
+End MessageConfig_def.
+
+Declare Scope mailbox_config_scope.
+
+Infix "=ᵐᵇ" := mailbox_eq (at level 71, left associativity) : mailbox_config_scope.
+Infix "⊎" := mailbox_union (at level 68, left associativity) : mailbox_config_scope.
+Notation "⟨ M ⟩" := (SingletonMailbox M).
+Notation "⟨⟩" := (EmptyMailbox).
+
+Open Scope mailbox_config_scope.
+
+(** ** Strings as messages *)
+Require Import String.
+Section StringMessages.
+
+Global Instance StringMessage : IMessage string :=
+{
+  message_eq_dec := string_dec
+}.
+
+End StringMessages.
+
+(** ** Example finite message set *)
+Section SendReceiveMessages.
+
+Inductive SendReceive : Type :=
+    Send : SendReceive
+  | Receive : SendReceive.
+
+Definition SendReceive_eq (m1 m2 : SendReceive) : Prop :=
+  match m1, m2 with
+  | Send, Send => True
+  | Receive, Receive => True
+  | _, _ => False
+  end.
+
+Instance SendReceive_eq_equiv : Equivalence SendReceive_eq.
+Proof.
+  constructor.
+  - unfold Reflexive; intros x; destruct x; now simpl.
+  - unfold Symmetric; intros x y Eq. destruct x; destruct y; simpl; simpl in Eq; auto.
+  - unfold Transitive; intros x y Eq1 Eq2; destruct x;
+    destruct y; destruct Eq1; destruct Eq2; auto.
+Qed.
+
+Lemma SendReceive_eq_dec : forall m n, {SendReceive_eq m n} + {~ SendReceive_eq m n}.
+Proof.
+  intros m n; destruct m; destruct n; simpl; auto.
+Defined.
+
+Global Instance SendReceiveMessage : IMessage SendReceive :=
+{
+  message_eq := SendReceive_eq;
+  message_eq_dec := SendReceive_eq_dec
+}.
+
+End SendReceiveMessages.
